ntruplus/proof/768/ref/poly_basemul_invntt/NTRUPlus768PolyBasemulInvNTTAlgebra.ec
@@ -1,0 +1,154 @@
+require import AllCore IntDiv Ring StdOrder.
+from Jasmin require import JWord JModel_x86.
+
+require import Array4 Array768.
+require import NTRUPlus768BasemulAlgebra.
+require import NTRUPlus768PolyBasemul.
+require import NTRUPlus768PolyBasemulProof.
+require import NTRUPlus768PolyBasemulAlgebra.
+require import NTRUPlus768InvNTTRadix2_4Algebra.
+require import NTRUPlus768InvNTTAlgebra.
+
+import Ring.IntID IntOrder.
+
+op poly_basemul_invntt_ready
+    (ap bp rp : W16.t Array768.t) : bool =
+  poly_basemul_qring ap bp rp 192 /\
+  NTRUPlus768InvNTTRadix2_4Algebra.qrange_input_shape rp.
+
+lemma in_qrange4_nth
+    (a : W16.t Array4.t) (j : int) :
+  in_qrange4 a =>
+  0 <= j < 4 =>
+  in_qrange a.[j].
+proof.
+  move=> Ha Hj.
+  move: Ha => [Ha0 [Ha1 [Ha2 Ha3]]].
+  have Hcases : j = 0 \/ j = 1 \/ j = 2 \/ j = 3 by smt().
+  elim Hcases => [-> | [-> | [-> | ->]]].
+  + exact Ha0.
+  + exact Ha1.
+  + exact Ha2.
+  exact Ha3.
+qed.
+
+lemma block4_nthE
+    (p : W16.t Array768.t) (k j : int) :
+  0 <= k < 192 =>
+  0 <= j < 4 =>
+  (block4 p k).[j] = p.[4 * k + j].
+proof.
+  move=> Hk Hj.
+  by rewrite /block4 Array4.initiE 1:/#.
+qed.
+
+lemma qring_block_output_qrange
+    (ap bp rp : W16.t Array768.t) (k : int) :
+  poly_basemul_qring ap bp rp 192 =>
+  0 <= k < 192 =>
+  in_qrange4 (block4 rp k).
+proof.
+  move=> Hqring Hk.
+  have Hblock := Hqring k Hk.
+  by move: Hblock => [Hrange _].
+qed.
+
+lemma blockwise_qrange4_implies_invntt_input_shape
+    (p : W16.t Array768.t) :
+  (forall k, 0 <= k < 192 => in_qrange4 (block4 p k)) =>
+  NTRUPlus768InvNTTRadix2_4Algebra.qrange_input_shape p.
+proof.
+  move=> Hblocks j Hj.
+  have Hk : 0 <= j %/ 4 < 192 by smt().
+  have Hj4 : 0 <= j %% 4 < 4 by smt().
+  have Hblock : in_qrange4 (block4 p (j %/ 4)).
+  + exact (Hblocks (j %/ 4) Hk).
+  have Hnth : in_qrange (block4 p (j %/ 4)).[j %% 4].
+  + exact (in_qrange4_nth (block4 p (j %/ 4)) (j %% 4) Hblock Hj4).
+  have -> : p.[j] = (block4 p (j %/ 4)).[j %% 4].
+  + rewrite (block4_nthE p (j %/ 4) (j %% 4) Hk Hj4).
+    have -> : 4 * (j %/ 4) + (j %% 4) = j by smt(edivzP).
+    done.
+  exact Hnth.
+qed.
+
+lemma in_qrange768_implies_invntt_input_shape
+    (p : W16.t Array768.t) :
+  in_qrange768 p =>
+  NTRUPlus768InvNTTRadix2_4Algebra.qrange_input_shape p.
+proof.
+  move=> Hp.
+  apply blockwise_qrange4_implies_invntt_input_shape.
+  exact Hp.
+qed.
+
+lemma poly_basemul_qring_implies_invntt_ready
+    (ap bp rp : W16.t Array768.t) :
+  poly_basemul_qring ap bp rp 192 =>
+  poly_basemul_invntt_ready ap bp rp.
+proof.
+  move=> Hqring.
+  split; first exact Hqring.
+  apply blockwise_qrange4_implies_invntt_input_shape.
+  by move=> k Hk; exact (qring_block_output_qrange ap bp rp k Hqring Hk).
+qed.
+
+lemma poly_basemul_qring_inverse_invntt_spec_algebra
+    (ap bp rp : W16.t Array768.t) :
+  poly_basemul_qring ap bp rp 192 =>
+  NTRUPlus768InvNTTAlgebra.inverse_invntt_algebra rp
+    (NTRUPlus768InvNTTAlgebra.inverse_invntt_spec rp).
+proof.
+  move=> Hqring.
+  have Hready := poly_basemul_qring_implies_invntt_ready ap bp rp Hqring.
+  move: Hready => [_ Hshape].
+  exact (NTRUPlus768InvNTTAlgebra.inverse_invntt_spec_algebra rp Hshape).
+qed.
+
+lemma poly_basemul_qring_inverse_invntt_output_qrange
+    (ap bp rp : W16.t Array768.t) (j : int) :
+  poly_basemul_qring ap bp rp 192 =>
+  0 <= j < 768 =>
+  -q <= coeff (NTRUPlus768InvNTTAlgebra.inverse_invntt_spec rp).[j] < q.
+proof.
+  move=> Hqring Hj.
+  have Hready := poly_basemul_qring_implies_invntt_ready ap bp rp Hqring.
+  move: Hready => [_ Hshape].
+  exact (NTRUPlus768InvNTTAlgebra.inverse_invntt_output_qrange rp j Hshape Hj).
+qed.
+
+lemma poly_basemul_correct_invntt_ready
+    (rp0 ap0 bp0 : W16.t Array768.t) :
+  in_s12range768 ap0 =>
+  in_s12range768 bp0 =>
+  phoare [NTRUPlus768PolyBasemul.M.jade_ntruplus_ntruplus768_amd64_ref_poly_basemul :
+    rp = rp0 /\ ap = ap0 /\ bp = bp0 ==>
+    poly_basemul_invntt_ready ap0 bp0 res] = 1%r.
+proof.
+  move=> Hap Hbp.
+  conseq poly_basemul_lossless (poly_basemul_functional rp0 ap0 bp0).
+  move=> &hr _ result; split.
+  + move=> [_ Hword].
+    split.
+    + trivial.
+    exact Hword.
+  move=> [_ Hword]; split.
+  + have Hqring :=
+      poly_basemul_word_to_qring_s12 ap0 bp0 result Hap Hbp Hword.
+    exact (poly_basemul_qring_implies_invntt_ready ap0 bp0 result Hqring).
+  exact Hword.
+qed.
+
+lemma poly_basemul_correct_invntt_ready_qrange
+    (rp0 ap0 bp0 : W16.t Array768.t) :
+  in_qrange768 ap0 =>
+  in_qrange768 bp0 =>
+  phoare [NTRUPlus768PolyBasemul.M.jade_ntruplus_ntruplus768_amd64_ref_poly_basemul :
+    rp = rp0 /\ ap = ap0 /\ bp = bp0 ==>
+    poly_basemul_invntt_ready ap0 bp0 res] = 1%r.
+proof.
+  move=> Hap Hbp.
+  exact (poly_basemul_correct_invntt_ready rp0 ap0 bp0
+    (in_qrange768_in_s12range768 ap0 Hap)
+    (in_qrange768_in_s12range768 bp0 Hbp)).
+qed.
